sf/Imp

sf/Imp.v
@@ -1609,37 +1609,67 @@ Inductive sinstr : Type :=
     malformed program. *)
 
 Fixpoint s_execute (st : state) (stack : list nat)
-                   (prog : list sinstr)
-                 : list nat
-  (* REPLACE THIS LINE WITH ":= _your_definition_ ." *). Admitted.
+         (prog : list sinstr)
+  : list nat :=
+  match prog with
+  | []            => stack
+  | (SPush x)::tl => s_execute st (x::stack) tl
+  | (SLoad n)::tl => s_execute st ((st n)::stack) tl
+  | SPlus::tl     =>
+    let ns := (match stack with
+               | [] => []
+               | [x] => [x]
+               | x::y::tl => (y + x)::tl
+               end)
+    in s_execute st ns tl
+  | SMinus::tl    =>
+    let ns := (match stack with
+               | [] => []
+               | [x] => [x]
+               | x::y::tl => (y - x)::tl
+               end)
+    in s_execute st ns tl
+  | SMult::tl     =>
+    let ns := (match stack with
+               | [] => []
+               | [x] => [x]
+               | x::y::tl => (y * x)::tl
+               end)
+    in s_execute st ns tl
+  end.
 
 Example s_execute1 :
      s_execute empty_state []
        [SPush 5; SPush 3; SPush 1; SMinus]
-   = [2; 5].
-(* FILL IN HERE *) Admitted.
+     = [2; 5].
+Proof. simpl. reflexivity. Qed.
 
 Example s_execute2 :
      s_execute (t_update empty_state X 3) [3;4]
        [SPush 4; SLoad X; SMult; SPlus]
-   = [15; 4].
-(* FILL IN HERE *) Admitted.
+     = [15; 4].
+Proof. simpl. reflexivity. Qed.
 
 (** Next, write a function that compiles an [aexp] into a stack
     machine program. The effect of running the program should be the
     same as pushing the value of the expression on the stack. *)
 
-Fixpoint s_compile (e : aexp) : list sinstr
-  (* REPLACE THIS LINE WITH ":= _your_definition_ ." *). Admitted.
+Fixpoint s_compile (e : aexp) : list sinstr :=
+  match e with
+  | ANum n => [SPush n]
+  | AId x  => [SLoad x]
+  | APlus e1 e2 => (s_compile e1) ++ (s_compile e2) ++ [SPlus]
+  | AMinus e1 e2 => (s_compile e1) ++ (s_compile e2) ++ [SMinus]
+  | AMult e1 e2 => (s_compile e1) ++ (s_compile e2) ++ [SMult]
+  end.
 
 (** After you've defined [s_compile], prove the following to test
     that it works. *)
 
 Example s_compile1 :
     s_compile (AMinus (AId X) (AMult (ANum 2) (AId Y)))
-  = [SLoad X; SPush 2; SLoad Y; SMult; SMinus].
-(* FILL IN HERE *) Admitted.
-(** [] *)
+    = [SLoad X; SPush 2; SLoad Y; SMult; SMinus].
+Proof. simpl. reflexivity. Qed.
 
 (** **** Exercise: 4 stars, advanced (stack_compiler_correct)  *)
 (** Now we'll prove the correctness of the compiler implemented in the
@@ -1653,13 +1683,15 @@ Example s_compile1 :
     more general lemma to get a usable induction hypothesis; the main
     theorem will then be a simple corollary of this lemma. *)
 
+Lemma s_execute_result : forall (st : state) (s : sinstr),
+     s  s_execute st [] (s_compile e) = 
 
 Theorem s_compile_correct : forall (st : state) (e : aexp),
   s_execute st [] (s_compile e) = [ aeval st e ].
 Proof.
-  (* FILL IN HERE *) Admitted.
-(** [] *)
-
+  intros. induction e; unfold s_compile; simpl; repeat reflexivity.
+  - fold s_compile. 
+  
 (** **** Exercise: 3 stars, optional (short_circuit)  *)
 (** Most modern programming languages use a "short-circuit" evaluation
     rule for boolean [and]: to evaluate [BAnd b1 b2], first evaluate
